ReducibilityDefinition.v
@@ -10,6 +10,7 @@ Require Import Coq.Classes.RelationClasses.
 
 Require Import Omega.
 
+(*
 Definition reduces_to (P: tree -> Prop) (t: tree) :=
   closed_term t /\
   exists v, P v /\ star scbv_step t v.
@@ -22,122 +23,123 @@ Lemma reduces_to_equiv:
 Proof.
   unfold reduces_to; repeat step; eauto.
 Qed.
+*)
 
-Equations (noind) reducible_values (theta: interpretation) (v: tree) (T: tree): Prop
+Equations (noind) reducible (theta: interpretation) (v: tree) (T: tree): Prop
     by wf (get_measure T) lt_measure :=
-  reducible_values theta v (fvar X type_var) :=
+  reducible theta v (fvar X type_var) :=
     match lookup Nat.eq_dec theta X with
     | None => False
     | Some P => P v
     end;
 
-  reducible_values theta v T_unit := v = uu;
+  reducible theta v T_unit := v = uu;
 
-  reducible_values theta v T_bool := v = ttrue \/ v = tfalse;
+  reducible theta v T_bool := v = ttrue \/ v = tfalse;
 
-  reducible_values theta v T_nat := is_nat_value v;
+  reducible theta v T_nat := is_nat_value v;
 
-  reducible_values theta v (T_abs T) :=
+  reducible theta v (T_abs T) :=
     closed_value v /\
     exists X,
       ~(X ∈ support theta) /\
       ~(X ∈ pfv T type_var) /\
       forall RC,
         reducibility_candidate RC ->
-        reducible_values ((X,RC) :: theta) v (topen 0 T (fvar X type_var));
+        reducible ((X,RC) :: theta) v (topen 0 T (fvar X type_var));
 
-  reducible_values theta v (T_arrow A B) :=
+  reducible theta v (T_arrow A B) :=
     exists (_: is_erased_type B),
     closed_value v /\
     forall a (p: is_erased_term a),
       wf a 0 ->
       pfv a term_var = nil ->
-      reducible_values theta a A ->
-      reduces_to (fun t => reducible_values theta t (open 0 B a)) (app v a);
+      reducible theta a A ->
+      reduces_to (fun t => reducible theta t (open 0 B a)) (app v a);
 
-  reducible_values theta v (T_prod A B) :=
+  reducible theta v (T_prod A B) :=
     exists (_: is_erased_type B),
     closed_value v /\
     exists a b (_: is_erased_term a),
       wf a 0 /\
       pfv a term_var = nil /\
       v = pp a b /\
-      reducible_values theta a A /\
-      reducible_values theta b (open 0 B a);
+      reducible theta a A /\
+      reducible theta b (open 0 B a);
 
-  reducible_values theta v (T_sum A B) :=
+  reducible theta v (T_sum A B) :=
     closed_value v /\ (
-      (exists v', v = tleft v' /\ reducible_values theta v' A) \/
-      (exists v', v = tright v' /\ reducible_values theta v' B)
+      (exists v', v = tleft v' /\ reducible theta v' A) \/
+      (exists v', v = tright v' /\ reducible theta v' B)
     );
 
-  reducible_values theta v (T_refine T p) :=
+  reducible theta v (T_refine T p) :=
     closed_value v /\
-    reducible_values theta v T /\
+    reducible theta v T /\
     is_erased_term p /\
     wf p 1 /\
     pfv p term_var = nil /\
     star scbv_step (open 0 p v) ttrue;
 
-  reducible_values theta v (T_type_refine T1 T2) :=
+  reducible theta v (T_type_refine T1 T2) :=
     exists (_: is_erased_type T2),
     exists (_: closed_value v),
-      reducible_values theta v T1 /\
-      exists p, reducible_values theta p (open 0 T2 v);
+      reducible theta v T1 /\
+      exists p, reducible theta p (open 0 T2 v);
 
-  reducible_values theta v (T_intersection A B) :=
+  reducible theta v (T_intersection A B) :=
     closed_value v /\
-    reducible_values theta v A /\
-    reducible_values theta v B;
+    reducible theta v A /\
+    reducible theta v B;
 
-  reducible_values theta v (T_union A B) :=
+  reducible theta v (T_union A B) :=
     closed_value v /\ (
-      reducible_values theta v A \/
-      reducible_values theta v B
+      reducible theta v A \/
+      reducible theta v B
     );
 
-  reducible_values theta v T_top :=
+  reducible theta v T_top :=
     closed_value v;
 
-  reducible_values theta v T_bot := False;
+  reducible theta v T_bot := False;
 
-  reducible_values theta v (T_equiv t1 t2) :=
+  reducible theta v (T_equiv t1 t2) :=
     v = uu /\
     equivalent_terms t1 t2;
 
-  reducible_values theta v (T_forall A B) :=
+  reducible theta v (T_forall A B) :=
     exists (_: is_erased_type B),
     closed_value v /\
     forall a (p: is_erased_term a),
       wf a 0 ->
       pfv a term_var = nil ->
-      reducible_values theta a A ->
-      reducible_values theta v (open 0 B a);
+      reducible theta a A ->
+      reducible theta v (open 0 B a);
 
-  reducible_values theta v (T_exists A B) :=
+  reducible theta v (T_exists A B) :=
     exists (_: is_erased_type B),
     closed_value v /\
     exists a (_: is_erased_term a),
       wf a 0 /\
       pfv a term_var = nil /\
-      reducible_values theta a A /\
-      reducible_values theta v (open 0 B a);
+      reducible theta a A /\
+      reducible theta v (open 0 B a);
 
-  reducible_values theta v (T_rec n T0 Ts) :=
+  reducible theta v (T_rec n T0 Ts) :=
     closed_value v /\
     is_erased_term n /\ (
-      (star scbv_step n zero /\ reducible_values theta v T0) \/
+      (star scbv_step n zero /\ reducible theta v T0) \/
       (exists n' X (p1: is_nat_value n') (p2: star scbv_step n (succ n')),
          ~(X ∈ pfv T0 type_var) /\
          ~(X ∈ pfv Ts type_var) /\
          ~(X ∈ support theta) /\
-         reducible_values ((X, fun t => reducible_values theta t (T_rec n' T0 Ts)) :: theta)
+         reducible ((X, fun t => reducible theta t (T_rec n' T0 Ts)) :: theta)
                           v
                           (topen 0 Ts (fvar X type_var))
       )
     );
 
-  reducible_values theta v T := False
+  reducible theta v T := False
 .
 
 Hint Transparent lt_measure: core.
@@ -151,18 +153,18 @@ Ltac reducibility_definition :=
 
 Solve Obligations with reducibility_definition.
 
-Fail Next Obligation. (* no more obligations for reducible_values *)
+Fail Next Obligation. (* no more obligations for reducible *)
 
 Definition reducible (theta: interpretation) t T : Prop :=
-  reduces_to (fun t => reducible_values theta t T) t.
+  reduces_to (fun t => reducible theta t T) t.
 
 Definition subtype theta T1 T2 :=
-  forall v, reducible_values theta v T1 -> reducible_values theta v T2.
+  forall v, reducible theta v T1 -> reducible theta v T2.
 
 Definition open_reducible (tvars: tvar_list) (gamma: context) t T : Prop :=
   forall theta lterms,
     valid_interpretation theta ->
-    satisfies (reducible_values theta) gamma lterms  ->
+    satisfies (reducible theta) gamma lterms  ->
     support theta = tvars ->
     reducible theta
               (substitute t lterms)
@@ -171,14 +173,14 @@ Definition open_reducible (tvars: tvar_list) (gamma: context) t T : Prop :=
 Definition open_subtype (tvars: tvar_list) (gamma: context) T1 T2 : Prop :=
   forall theta l,
    valid_interpretation theta ->
-   satisfies (reducible_values theta) gamma l ->
+   satisfies (reducible theta) gamma l ->
    support theta = tvars ->
    subtype theta (substitute T1 l) (substitute T2 l).
 
 Definition open_equivalent (tvars: tvar_list) (gamma: context) t1 t2 : Prop :=
   forall theta l,
     valid_interpretation theta ->
-    satisfies (reducible_values theta) gamma l ->
+    satisfies (reducible theta) gamma l ->
     support theta = tvars ->
     equivalent_terms (substitute t1 l) (substitute t2 l).
 
@@ -193,7 +195,7 @@ Notation "'[' tvars ';' gamma '⊨' t1 '≡' t2 ']'" := (open_equivalent tvars g
 
 Lemma reducibility_rewrite:
   forall theta t T,
-    reduces_to (fun t => reducible_values theta t T) t =
+    reduces_to (fun t => reducible theta t T) t =
     reducible theta t T.
 Proof.
   reflexivity.
@@ -212,19 +214,19 @@ Qed.
 
 Ltac simp_red_hyp :=
   match goal with
-  | H: _ |- _ => rewrite_strat outermost hints reducible_values in H
+  | H: _ |- _ => rewrite_strat outermost hints reducible in H
   end.
 
 Ltac simp_red_top_level_hyp :=
   match goal with
-  | H: _ |- _ => rewrite_strat hints reducible_values in H
+  | H: _ |- _ => rewrite_strat hints reducible in H
   end.
 
-Ltac simp_red_goal := rewrite_strat outermost hints reducible_values.
+Ltac simp_red_goal := rewrite_strat outermost hints reducible.
 
 Ltac simp_red := simp_red_hyp || simp_red_goal.
 
 Ltac simp_red_nat :=
   match goal with
-  | H: reducible_values _ _ T_nat |- _ => simp reducible_values in H
+  | H: reducible _ _ T_nat |- _ => simp reducible in H
   end.
